add quotient type

QuotientType.v
@@ -14,6 +14,22 @@ Qed.
 Definition PFE l r := l mod 5 = r mod 5.
 Definition MF := quotient PFE.
 Definition mk_MF (n : nat) : MF := mk_quotient PFE n.
+
+Definition of_nat_lt_eq n lv lp rv rp :
+  lv = rv -> @Fin.of_nat_lt lv n lp = @Fin.of_nat_lt rv n rp.
+  intros; subst; f_equal; apply proof_irrelevance.
+Qed.
+
+Program Definition toFin (l : MF) : Fin.t 5 := 
+  l (Fin.t 5) (fun n => @Fin.of_nat_lt (n mod 5) _ _) _.
+Next Obligation.
+  repeat match_destruct; omega.
+Defined.
+Next Obligation.
+  apply of_nat_lt_eq.
+  compute in *; trivial.
+Defined.
+
 Program Definition MFPlus (l r : MF) : MF := 
   l MF (fun ln => r MF (fun rn => mk_MF (ln + rn)) _) 
     (fun _ _ _ => quotient_elim_eq _ _ _ _).
@@ -21,8 +37,28 @@ Next Obligation.
   unfold mk_MF, mk_quotient, PFE in *; repeat ext.
   apply H2.
   rewrite (Nat.add_mod ln l0), (Nat.add_mod ln r0); f_equal; omega.
-Defined.
+Qed.
 Next Obligation.
   ext; apply EQ_eq; unfold PFE in *.
   rewrite (Nat.add_mod H), (Nat.add_mod H0); f_equal; omega.
-Defined.
+Qed.
+
+Program Definition MFMult (l r : MF) : MF := 
+  l MF (fun ln => r MF (fun rn => mk_MF (ln * rn)) _) 
+    (fun _ _ _ => quotient_elim_eq _ _ _ _).
+Next Obligation.
+  unfold mk_MF, mk_quotient, PFE in *; repeat ext.
+  apply H2.
+  rewrite (Nat.mul_mod ln l0), (Nat.mul_mod ln r0); do 2 f_equal; omega.
+Qed.
+Next Obligation.
+  ext; apply EQ_eq; unfold PFE in *.
+  rewrite (Nat.mul_mod H), (Nat.mul_mod H0); do 2 f_equal; omega.
+Qed.
+
+Program Definition Evil (l : MF) : nat := l nat id _.
+Next Obligation.
+Admitted.
+
+Eval compute in toFin (MFPlus (mk_MF 4) (mk_MF 7)).
+Eval compute in Evil (MFPlus (mk_MF 4) (mk_MF 7)).
